theories/stack.v
@@ -1,3 +1,4 @@
+From stdpp Require Import sorting.
 From iris.proofmode Require Import tactics.
 From iris.algebra Require Import excl auth list frac_auth gmap gset.
 From iris.base_logic.lib Require Import invariants.
@@ -15,62 +16,252 @@ Section stack_stuff.
   Proof. apply _. Qed.
   Global Instance stack_cont_timeless l γ : Timeless (stack_cont l γ).
   Proof. apply _. Qed.
+  Global Instance to_val_inj : Inj (=) (=) to_val.
+  Proof. intros l1 l2 H. case l1, l2; try done. inversion H. reflexivity. Qed.
   Typeclasses Opaque is_stack stack_cont.
 End stack_stuff.
+Local Hint Extern 0 (environments.envs_entails _ (phys_stack _ [])) => iExists None : core.
+Local Hint Extern 0 (environments.envs_entails _ (phys_stack _ (_ :: _))) => iExists (Some _) : core.
+Local Hint Extern 10 (environments.envs_entails _ (phys_stack _ _)) => unfold phys_stack : core.
+Local Hint Extern 0 (environments.envs_entails _ (phys_list None [])) => simpl : core.
+Local Hint Extern 0 (environments.envs_entails _ (phys_list (Some _) (_ :: _))) => simpl : core.
 
-Section operation.
+(* NOTE: iFrame may fail for Opaque definitions  *)
+Typeclasses Transparent hist hist_snap stack_cont.
+Section spec.
   Inductive stack_op := Push of val | Pop of val.
   Canonical Structure stack_opO := leibnizO stack_op.
-  (* TODO: linearizability stuff *)
-End operation.
+  Definition Hist := @Hist stack_opO.
 
-Section spec.
   Context `{!heapG Σ, !stackG Σ, !@histG stack_opO Σ} (N : namespace).
 
-  Definition stackN := nroot .@ "stack".
-  Notation is_stack := (is_stack stackN).
+  Definition stack_hist_entry_le : relation (nat * excl stack_op) :=
+    λ (x y : (nat * excl stack_op)), x.1 <= y.1.
+  Instance stack_hist_entry_le_dec : RelDecision stack_hist_entry_le.
+  Proof. refine (λ (x y : (nat * excl stack_op)), decide ((x.1 ?= y.1) ≠ Gt)). Qed.
 
-  Definition stack_histN := nroot .@ "stack_hist".
-  Definition stack_hist γh := inv stack_histN (∃ hs t, hist γh hs t).
+  Fixpoint stack_hist_cont_aux s (hs : list (nat * excl stack_op)) : option (list val) :=
+    match hs with
+    | [] => Some s
+    | (_, ExclBot) :: _ => None
+    | (_, Excl (Push v)) :: hs' => stack_hist_cont_aux (v :: s) hs'
+    | (_, Excl (Pop v)) :: hs' =>
+      match s with
+      | [] => None
+      | v' :: s' => if decide (v = v') then stack_hist_cont_aux s' hs' else None
+      end
+    end.
+
+  Definition stack_hist_cont (hs : Hist) : option (list val) :=
+    stack_hist_cont_aux [] $ merge_sort stack_hist_entry_le $ gmap_to_list hs .
+
+  (* Fixpoint stack_hist_cont_aux (hs : Hist) s l : option (list val) :=
+       match l with
+       | O => Some s
+       | S l' =>
+         match hs !! l' with
+         | None => None
+         | Some ExclBot => None
+         | Some (Excl (Push v)) => stack_hist_cont_aux hs (v :: s) l'
+         | Some (Excl (Pop v)) =>
+           match s with
+           | [] => None
+           | v' :: s' => if decide (v = v') then stack_hist_cont_aux hs s' l' else None
+           end
+         end
+       end.
+
+     Definition stack_hist_cont hs l : option (list val) :=
+       stack_hist_cont_aux hs [] l. *)
+
+  Lemma stack_hist_cont_empty : stack_hist_cont ε = Some [].
+  Proof. by vm_compute. Qed.
+
+  Lemma stack_hist_cont_push t hs v xs:
+    hist_gapless t hs ->
+    stack_hist_cont hs = Some xs ->
+    stack_hist_cont (<[t:=Excl (Push v)]> hs) = Some (v::xs).
+  Proof.
+  Admitted.
+
+  Lemma stack_hist_cont_pop t hs v xs:
+    hist_gapless t hs ->
+    stack_hist_cont hs = Some (v::xs) ->
+    stack_hist_cont (<[t:=Excl (Pop v)]> hs) = Some xs.
+  Proof.
+  Admitted.
+
+  (* TODO: need to track last timestamp? *)
+  Definition stack_hist γs γh l :=
+    inv N (∃ hs t xs, phys_stack l xs ∗ own γs (● Excl' xs) ∗
+                      hist γh hs t ∗ ⌜stack_hist_cont hs = Some xs⌝).
+
+  (* impossible? stack_hist γs γh l -∗ is_stack γs l. *)
+
+  (* TODO: what rel for stack_cont and hist_snap? *)
+  Definition stack_hist_snap γs γh q xs hs : iProp Σ :=
+    stack_cont γs xs ∗
+    hist_snap γh q hs ∗
+    ⌜∃ hsM tM, hs ≼ hsM ∧ hist_gapless tM hsM ∧ stack_hist_cont hsM = Some xs⌝.
 
   Lemma new_stack_spec_hist :
     {{{ True }}}
       new_stack #()
-    {{{ l γs γh, RET #l; is_stack l γs ∗ stack_cont γs [] ∗ stack_hist γh ∗ hist_snap γh 1 ε }}}.
+    {{{ l γs γh, RET #l; stack_hist γs γh l ∗ stack_hist_snap γs γh 1 [] ε }}}.
   Proof.
-    iIntros (Φ) "_ Post".
+    iIntros (Φ) "_ HΦ".
     iApply wp_fupd.
-    iMod hist_alloc as (γh) "[Hγh● Hγh◯]".
-    iMod (inv_alloc stack_histN _ (∃ hs t, hist γh hs t) with "[Hγh●]") as "Hist"; first eauto.
-    wp_apply (new_stack_spec stackN); first done.
-    iIntros (l γs) "[Stack Sc] !>". iApply "Post". iFrame.
+    wp_lam. wp_alloc l as "Hl".
+    iMod (own_alloc (● (Excl' []) ⋅ ◯ (Excl' []))) as (γs) "[Hs● Hs◯]";
+      first by apply auth_both_valid.
+    iMod hist_alloc as (γh) "[Hh● Hh◯]".
+    iMod (inv_alloc N _
+                    (∃ (hs : Hist) t xs,
+                        phys_stack l xs ∗ own γs (● Excl' xs) ∗
+                        hist γh hs t ∗ ⌜stack_hist_cont hs = Some xs⌝)
+            with "[Hl Hs● Hh●]").
+    { iNext; iExists ε, O, []. iFrame. iSplitL "Hl". eauto with iFrame.
+      iPureIntro. apply stack_hist_cont_empty. }
+    iModIntro. iApply "HΦ". iFrame. iPureIntro. by exists ε, O.
   Qed.
 
+
   Lemma push_stack_spec_hist (l : loc) (γs γh : gname) (v : val) :
-    is_stack l γs -∗ stack_hist γh -∗
-    <<< ∀ xs q hs, stack_cont γs xs ∗ hist_snap γh q hs >>>
-      push_stack v #l @ ⊤ ∖ ↑stackN ∖ ↑stack_histN
-    <<< ∃ t, stack_cont γs (v::xs) ∗ hist_snap γh q (<[t := Excl (Push v)]> hs ), RET #() >>>.
+    stack_hist γs γh l -∗
+    <<< ∀ xs q hs, stack_hist_snap γs γh q xs hs >>>
+      push_stack v #l @ ⊤ ∖ ↑N
+    <<< ∃ (t:nat), stack_hist_snap γs γh q (v::xs) (<[t := Excl (Push v)]> hs) ∗
+                 ⌜∀ (t':nat), t' ∈ (dom (gset nat) hs) → t' < t⌝,
+        RET #() >>>.
   Proof.
-    iIntros "#Stack #Hist" (Φ) "AU".
-    awp_apply (push_stack_spec stackN with "Stack").
-    iInv stack_histN as (hsM tM) ">Hh".
-    iApply (aacc_aupd_commit with "AU"); first solve_ndisj.
-    iIntros (xs q hs) "[Hsc Hhs]".
-    iAaccIntro with "Hsc"; first by auto 10 with iFrame.
-    iMod (hist_update γh q hsM hs tM (Push v) with "Hh Hhs") as "[Hh Hhs]".
-    eauto 11 with iFrame.
+    iIntros "#SH" (Φ) "AU". iLöb as "IH".
+    wp_lam; wp_let; wp_bind (! _)%E.
+    iInv "SH" as (hsM tM xs) ">(HPhys & Hs● & Hh● & %)". rename H0 into Hcont.
+    iDestruct "HPhys" as (w) "[Hl HPhys]".
+    wp_load. iModIntro. iSplitR "AU"; first by eauto 10 with iFrame.
+    clear Hcont hsM tM xs.
+
+    wp_alloc r as "Hr". wp_inj. wp_bind (CmpXchg _ _ _)%E.
+    iInv "SH" as (hsM tM ys) ">(HPhys & Hs● & Hh● & %)". rename H0 into Hcont.
+    iDestruct "HPhys" as (u) "[Hl HPhys]".
+    destruct (decide (u = w)) as [[= ->]|NE].
+    - wp_cmpxchg_suc; first by case w; left. (* TODO: solve_vals_compare_safe doesn't work *)
+      iMod "AU" as (zs q hs) "[(Hs◯ & Hh◯ & %) [_ HClose]]". rename H0 into Hcont_frag.
+      iDestruct (auth_agree with "Hs● Hs◯") as %->.
+
+      (* TODO: just to extract pure stuff. simpler solution? *)
+      iDestruct "Hh●" as "[Hh● Hg]". iDestruct "Hg" as %Hg.
+      iAssert (⌜hist_gapless tM hsM⌝)%I as "Hg"; first done.
+      iDestruct (own_valid_2 with "Hh● Hh◯") as %Hincl%frac_auth_included_total.
+      iCombine "Hh●" "Hg" as "Hh●". iClear "Hg".
+
+      iMod (auth_update γs (v::zs) with "Hs● Hs◯") as "[Hs● Hs◯]".
+      iMod (hist_update γh q hsM hs tM (Push v) with "Hh● Hh◯") as "[Hh● Hh◯]".
+      rewrite /stack_hist_snap /hist /hist_snap.
+      iDestruct "Hh●" as "[Hh● %]". rename H0 into Hg'.
+      set hsM' := <[tM:=Excl (Push v)]> hsM.
+      set hs' := <[tM:=Excl (Push v)]> hs.
+      (* pure assertions to close AU *)
+      iDestruct (own_valid_2 with "Hh● Hh◯") as %Hincl'%frac_auth_included_total.
+      assert (stack_hist_cont hsM' = Some (v :: zs)) as Hcont' by by apply stack_hist_cont_push.
+      assert (∀ t' : nat, t' ∈ dom (gset nat) hs → t' < tM).
+      { inversion Hg as [_ Hdom_hsM]. apply (dom_included hs hsM) in Hincl. intros t' Ht'.
+        rewrite ->(elem_of_subseteq) in Hincl. specialize (Hincl t' Ht'). apply Hdom_hsM in Hincl. lia. }
+      iMod ("HClose" with "[Hs◯ Hh◯]") as "HΦ".
+      iFrame. iPureIntro. split; [by exists hsM', (S tM) | done].
+      iModIntro. iSplitR "HΦ". (* TODO: cleanup *)
+      + iModIntro. iExists hsM', (S tM), (v::zs). iFrame "∗ %". iExists (Some r). iFrame. simpl.
+        iExists w. iFrame. iExists 1%Qp. iFrame.
+      + by wp_pures.
+    - wp_cmpxchg_fail.
+      { exact: not_inj. }
+      { case u, w; simpl; eauto. }
+      iModIntro. iSplitL "Hs● Hh● Hl HPhys"; first by eauto 10 with iFrame.
+      wp_pures. iApply "IH". iExact "AU".
   Qed.
 
   Lemma pop_stack_spec (l : loc) (γs γh : gname) :
-    is_stack l γs -∗ stack_hist γh -∗
-    <<< ∀ q hs, hist_snap γh q hs >>>
-      pop_stack #l @ ⊤ ∖ ↑stackN ∖ ↑stack_histN
-    <<< ∃ t, hist_snap γh q (<[ t := Excl (Pop #()) ]> hs ), RET #() >>>.
-    (* <<< stack_cont γs (match xs with [] => [] | _::xs => xs end)
-         , RET (match xs with [] => NONEV | v::_ => SOMEV v end) >>>. *)
+    stack_hist γs γh l -∗
+    <<< ∀ xs q hs, stack_hist_snap γs γh q xs hs >>>
+      pop_stack #l @ ⊤ ∖ ↑N
+    <<< match xs with
+        | [] => stack_hist_snap γs γh q [] hs
+        | v::xs' => ∃ (t:nat), stack_hist_snap γs γh q (xs') (<[t := Excl (Pop v)]> hs) ∗
+                 ⌜∀ (t':nat), t' ∈ (dom (gset nat) hs) → t' < t⌝
+        end,
+        RET match xs with
+            | [] => NONEV
+            | v::_ => SOMEV v
+            end >>>.
   Proof.
-  Admitted.
+    iIntros "#SH" (Φ) "AU". iLöb as "IH". wp_lam. wp_bind (! _)%E.
+    iInv "SH" as (hsM tM xs) ">(HPhys & Hs● & Hh● & %)". rename H0 into Hcont.
+    iDestruct "HPhys" as (w) "[Hl HPhys]".
+    wp_load.
+    iDestruct (phys_list_dup with "HPhys") as "[HPhys1 HPhys2]".
+    destruct w as [w|], xs as [|x xs]; try done; simpl.
+    - (* non-empty stack *)
+      iModIntro. iSplitL "Hl Hs● Hh● HPhys1"; first by eauto 10 with iFrame.
+      clear Hcont hsM tM.
+      wp_let. wp_match. iDestruct "HPhys2" as (r wq) "[Hw HP]".
+      wp_load. wp_let. wp_proj. wp_bind (CmpXchg _ _ _)%E.
+      iInv "SH" as (hsM tM ys) ">(HPhys & Hs● & Hh● & %)". rename H0 into Hcont.
+      iDestruct "HPhys" as (u) "[Hl HPhys]".
+      iClear "HP". clear xs.
+      destruct (decide (u = Some w)) as [[= ->]|Hx].
+      + wp_cmpxchg_suc.
+        destruct ys; first done.
+        iMod "AU" as (zs q hs) "[(Hs◯ & Hh◯ & %) [_ HClose]]". rename H0 into Hcont_frag.
+
+        (* TODO: extracting pure stuff *)
+        iDestruct "Hh●" as "[Hh● Hg]". iDestruct "Hg" as %Hg.
+        iAssert (⌜hist_gapless tM hsM⌝)%I as "Hg"; first done.
+        iDestruct (own_valid_2 with "Hh● Hh◯") as %Hincl%frac_auth_included_total.
+        iCombine "Hh●" "Hg" as "Hh●". iClear "Hg".
+
+        iDestruct (auth_agree with "Hs● Hs◯") as %<-.
+        iMod (auth_update γs ys with "Hs● Hs◯") as "[Hs● Hs◯]".
+        iDestruct "HPhys" as (u wq') "[Hw' HPhys]".
+        iDestruct (mapsto_agree with "Hw Hw'") as %[=-> ->%to_val_inj].
+
+        iMod (hist_update γh q hsM hs tM (Pop v) with "Hh● Hh◯") as "[Hh● Hh◯]".
+        iDestruct "Hh●" as "[Hh● %]". rename H0 into Hg'.
+        set hsM' := <[tM:=Excl (Pop v)]> hsM.
+        set hs' := <[tM:=Excl (Pop v)]> hs.
+
+        (* pure assertions to close AU *)
+        rewrite /stack_hist_snap /hist /hist_snap /stack_cont.
+        iDestruct (own_valid_2 with "Hh● Hh◯") as %Hincl'%frac_auth_included_total.
+        assert (stack_hist_cont hsM' = Some ys) as Hcont' by by apply stack_hist_cont_pop.
+        assert (∀ t' : nat, t' ∈ dom (gset nat) hs → t' < tM).
+        { inversion Hg as [_ Hdom_hsM]. apply (dom_included hs hsM) in Hincl. intros t' Ht'.
+          rewrite ->(elem_of_subseteq) in Hincl. specialize (Hincl t' Ht'). apply Hdom_hsM in Hincl. lia. }
+
+        iMod ("HClose" with "[Hs◯ Hh◯]") as "HΦ".
+        iExists tM. iFrame. iPureIntro. split; [by exists hsM', (S tM) | done].
+        iModIntro. iSplitR "HΦ". (* TODO: cleanup *)
+        * iModIntro. iExists hsM', (S tM), ys. iFrame "∗ %". unfold phys_stack. iExists u. iFrame.
+        * by wp_pures.
+      + wp_cmpxchg_fail.
+        { intro Heq. apply Hx. destruct u; inversion Heq; done. }
+        iModIntro. iSplitR "AU"; first by eauto 10 with iFrame.
+        wp_pures. iApply "IH". iExact "AU".
+    - (* empty stack *)
+      iClear "HPhys1 HPhys2".
+      iMod "AU" as (zs q hs) "[(Hs◯ & Hh◯ & %) [_ HClose]]". rename H0 into Hcont_frag. (* TODO: Hcont_frag not needed? *)
+      (* TODO: extracting pure stuff *)
+      iDestruct "Hh●" as "[Hh● Hg]". iDestruct "Hg" as %Hg.
+      iAssert (⌜hist_gapless tM hsM⌝)%I as "Hg"; first done.
+      iDestruct (own_valid_2 with "Hh● Hh◯") as %Hincl%frac_auth_included_total.
+      iCombine "Hh●" "Hg" as "Hh●". iClear "Hg".
+
+      iDestruct (auth_agree with "Hs● Hs◯") as %<-.
+      iMod ("HClose" with "[Hs◯ Hh◯]") as "HΦ".
+      { iFrame. by iExists hsM, tM. }
+      iModIntro. iSplitR "HΦ"; first by eauto 10 with iFrame.
+      wp_pures. iExact "HΦ".
+  Qed.
+
 End spec.
 
 From iris.heap_lang Require Import lib.par.
@@ -94,6 +285,7 @@ Module client.
   Definition exchange (s ap ac : loc) : val :=
     λ: "n", (produce s ap) "n" #0 ||| (consume s ac) "n" #0.
 
-  (* ap ↦∗ ls ∗ ∃ ls', ac ↦∗ ls' ∗ ⌜Permutation ls ls'⌝ *)
+  (* ap ↦∗ ls ∗ ∃ ls', ac ↦∗ ls' ∗ ⌜Permutation ls ls'⌝
+     hist_snap γh 1 hs, pushed hs l1, popped hs l2 -> Permutation l1 l2*)
 
 End client.
